---
solver: "Ileumassamuel"
date: "2021-08-30"
exerciseNumber: "1-12"

edition: "4"
author: "Michael Spivak"
textbook: "Calculus"
---

Prove the following:

(i) Proof by cases/exhaustion:

$\bm{x, y \geq 0}$ 
$$
\begin{aligned}
\wedge
[ \; x \geq 0 \wedge y \geq 0 \implies x = |x| \wedge y = |y| \; ] \\
& \implies |xy| = xy = |x| \cdot |y|
\end{aligned}
$$


$\bm{x, y \leq 0}$ 
$$
\begin{aligned}
\wedge
[ \; x \leq 0 \wedge y \leq 0 \implies -x = |x| \wedge -y = |y| \; ] \\
& \implies |xy| = xy = -x \cdot -y = |x| \cdot |y|
\end{aligned}
$$


$\bm{x \geq 0, y \leq 0}$ 
$$
\begin{aligned}
\\
\wedge \\
[ \; x \geq 0 \wedge y \leq 0 \implies x = |x| \wedge -y = |y| \; ] \\
\implies |xy| = x \cdot -y = |x| \cdot |y|
\end{aligned}
$$


We can ignore the case $x \leq 0, y \geq 0$ as it would be treated
by the third one, if the starting inequalities' variables were
interchanged.

(ii) 
$$
\begin{aligned}
|\frac{1}{x}| & = |1 \cdot x^{-1}| \\
& = |1| \cdot |x^{-1}| && (i) \\
& = 1 \cdot |x^{-1}| \\
& = \frac{1}{|x|}
\end{aligned}
$$


(iii) 
$$
\begin{aligned}
\frac{|x|}{|y|} & = |x| |y|^{-1} \\
& = |x| |y^{-1}| && (ii) \\
& = |\frac{x}{y}| && (i)
\end{aligned}
$$


(iv) 
$$
\begin{aligned}
|x  + z| \leq |x| + |z| & \implies |x + z| \leq |x| + |-z| && z = -y \\
& \implies |x + (-y)|  \leq |x| + |y| \\
& \implies |x - y| \leq |x| + |y|
\end{aligned}
$$


(v) 
$$
\begin{aligned}
|x| = |(x - y) + y| & \leq |x - y| + |y| && \text{Triangle inequality} \\
\implies |x| - |y| & \leq |x - y|
\end{aligned}
$$


(vi) 
$$
\begin{aligned}
|x| - |y| \leq |x - y| & \implies |y| - |x| \leq |y - x| && \text{Interchanging } x, y \\
& \implies |y| - |x| \leq |-(x - y)| \\
& \implies |y| - |x| \leq |x - y| \\
& \implies -|x - y| \ leq |x| - |y| \\
& \implies -|x - y| \leq |x| - |y| \leq |x - y| && (v) \\
& \implies ||x| - |y|| \leq |x - y|
\end{aligned}
$$


(vii) 
$$
\begin{aligned}
|x + y| \leq |x| + |y| \implies |x + y| + |z| & \leq |x| + |y| + |z| && \text{Triangle inequality} \\
\implies |(x + y) + z| \leq |x + y| + |z| & \leq |x| + |y| + |z|
\end{aligned}
$$
