---
solver: "Ileumassamuel"
date: "2021-08-30"
exerciseNumber: "1-13"

edition: "4"
author: "Michael Spivak"
textbook: "Calculus"
---

Geometrically, the formulae make perfect sense. Of
course, intuition is no substitute for a formal proof. **Let us start by
proving the max function**:

-   **If** $\bm{x \leq y}$ 
$$
\begin{aligned}
x \leq y & \implies y - x \geq 0 \\
& \implies \max{(x, y)} = \frac{x + y + (y - x)}{2} \\
& \implies \max({x, y}) = \frac{2y}{2} = y
\end{aligned}
$$


-   **If** $\bm{y \leq x}$ 
$$
\begin{aligned}
y \leq x & \implies y - x \leq 0 \\
& \implies \max{(x, y)} = \frac{x + y - (y - x)}{2} \\
& \implies \max{(x, y)} = \frac{2x}{2} = x
\end{aligned}
$$


**To prove the min function**:

-   **If** $\bm{x \leq y}$ 
$$
\begin{aligned}
x \leq y & \implies y - x \geq 0 \\
& \implies \min{(x, y)} = \frac{x + y - (y - x)}{2} \\
& \implies \min({x, y}) = \frac{2x}{2} = x
\end{aligned}
$$


-   **If** $\bm{y \leq x}$ 
$$
\begin{aligned}
y \leq x & \implies y - x \leq 0 \\
& \implies \min{(x, y)} = \frac{x + y - (- (y - x))}{2} \\
& \implies \min{(x, y)} = \frac{x + y + (y - x)}{2} \\
& \implies \min{(x, y)} = \frac{2y}{2} = y
\end{aligned}
$$
