---
solver: "Ileumassamuel"
date: "2021-08-30"
exerciseNumber: "1-15"

edition: "4"
author: "Michael Spivak"
textbook: "Calculus"
---

**We can prove the first inequality with a proof by
contradiction**. 
$$
\begin{aligned}
x^{2} + xy + y^{2} \leq 0 & \implies x^{2} + 2xy + y^{2} - xy \leq 0 \\
& \implies {(x + y)}^{2} - xy \leq 0 \\
& \implies {(x + y)}^{2} \leq xy
\end{aligned}
$$


Now, if $x > 0, y < 0$, we then obtain $xy < 0$. Consequently, we would
obtain the following contradiction. 
$$
\begin{aligned}
{(x + y)}^{2} \leq xy < 0 & \implies {(x + y)}^{2} < 0
\end{aligned}
$$


Notice, for the second inequality, that the polynomial can be factored.
Based on problem 1.4, 
$$
\begin{aligned}
\frac{x^{5} - y^{5}}{x - y} = x^{4} + x^{3}y + x^{2}y^{2} + xy^{3} + y^{4}
\end{aligned}
$$


**If** $\bm{x - y < 0}$: 
$$
\begin{aligned}
x - y < 0 & \implies x < y \\
& \implies x^{5} < y^{5} && (6.1) \\
& \implies x^{5} - y^{5} < 0 \\
& \implies \frac{x^{5} - y^{5}}{x - y} > 0
\end{aligned}
$$


On the other hand, **if** $\bm{x - y > 0}$ 
$$
\begin{aligned}
x - y > 0 & \implies x > y \\
& \implies x^{5} > y^{5} && (6.1) \\
& \implies x^{5} - y^{5} > 0 \\
& \implies \frac{x^{5} - y^{5}}{x - y} > 0
\end{aligned}
$$


As seen above, in both cases the fraction is greater than 0 and thus so
too is our polynomial.
