---
solver: "Ileumassamuel"
date: "2021-08-30"
exerciseNumber: "1-16"

edition: "4"
author: "Michael Spivak"
textbook: "Calculus"
---

(a) **For the first biconditional**, we start by decomposing the
left-hand side of the equation. 
$$
\begin{aligned}
{(x + y)}^{2} &= (x + y)(x + y) \\
&= x(x + y) + y(x + y) \\
&= x^{2} + xy + yx + y^{2} \\
& = x^{2} + 2xy + y^{2} && (1)
\end{aligned}
$$


We then equal it to the right-hand side of the equation:

$$
\begin{aligned}
x^{2} + 2xy + y^{2} = x^{2} + y^{2} & \iff 2xy = 0 && (1) \\
& \iff xy = 0 \\
& \iff x = 0 \; \vee \; y = 0
\end{aligned}
$$


**For the second biconditional**, we prove it the same way.

$$
\begin{aligned}
{(x + y)}^{3} &= (x + y)(x + y)(x + y) \\
&= (x + y)(x^{2} + 2xy + y^{2}) \\ 
&= x(x^{2} + 2xy + y^{2} + y(x^{2} + 2xy + y^{2} \\
&= x^{3} + 2x^{2}y + xy^{2} + yx^{2} + 2xy^{2} + y^{3} \\
&= x^{3} + 3x^{2}y + 3xy^{2} + y^{3} && (2)
\end{aligned}
$$


Again, we equate it to its right-hand side of the original equation:

$$
\begin{aligned}
x^{3} + 3x^{2}y + 3xy^{2} + y^{3} = x^{3} + y^{3} & \iff 3x^{2}y + 3xy^{2} = 0 && (2) \\
& \iff x^{2}y + xy^{2} = 0 \\
& \iff xy(x + y) = 0 \\
& \iff x = 0 \; \vee \; y = 0 \; \vee \; x + y = 0 \\
& \iff x = 0 \; \vee \; y = 0 \; \vee \; x = -y
\end{aligned}
$$


(b) We are going to prove this by contradiction. Assume, instead, that:

$$
\begin{aligned}
4x^{2} + 6xy + 4y^{2} < 0 & \implies 4x^{2} + 8xy + 4y^{2} - 2xy < 0 \\
& \implies {(2x + 2y)}^{2} - 2xy < 0 && \text{Square completion} \\
& \implies 4{(x + y)}^{2} < 2xy \\
& \implies 2{(x + y)}^{2} < xy
\end{aligned}
$$


Now, if we were to set one variable positive and the other negative,
we would obtain a negative product. That is, if $x > 0$ and $y < 0$,
then $xy < 0$ and consequently: 
$$
\begin{aligned}
2{(x + y)}^{2} < xy \; \wedge \; xy < 0 & \implies 2{(x + y)}^{2} < 0 \\
& \implies {(x + y)}^{2} < 0
\end{aligned}
$$


We thus end up with a contradiction. We can then that only the
opposite of our inequality holds: 
$$
\begin{aligned}
4x^{2} + 6xy + 4y^{2} \geq 0
\end{aligned}
$$


As asked, we also are to prove that the inequality does not hold
when $x$ and $y$ both are 0. 
$$
\begin{aligned}
x = 0 \; \wedge \; y = 0 & \implies x^{2} = 0 \; \wedge \; y^{2} \; \wedge \; xy = 0 \\
& \implies 4x^{2} = 0 \; \wedge \; 4y^{2} \; \wedge \; 6xy = 0 \\
& \implies 4x^{2} + 6xy + 4y^{2} = 0
\end{aligned}
$$


(c) 
$$
\begin{aligned}
{(x + y)}^{4} &= (x + y)(x^{3} + 3x^{2}y + 3xy^{2} + y^{3}) \\
&= x (x^{3} + 3x^{2}y + 3xy^{2} + y^{3}) + y (x^{3} + 3x^{2}y + 3xy^{2} + y^{3}) \\
&= x^{4} + 3x^{3}y + 3x^{2}y^{2} + xy^{3} + yx^{3} + 3x^{2}y^{2} + 3xy^{3} + y^{4} \\
&= x^{4} + 4x^{3}y + 4xy^{3} + 6x^{2}y^{2} + y^{4}
\end{aligned}
$$


We equate it to the right-hand side of the equation:

$$
\begin{aligned}
x^{4} + 4x^{3}y + 4xy^{3} + 6x^{2}y^{2} + y^{4} = x^{4} + y^{4} & \implies 4x^{3}y + 4xy^{3} + 6x^{2}y^{2} = 0 \\
& \implies xy(4x^{2} + 4y^{2} + 6xy) = 0 \\
& \implies x = 0 \; \vee \; y = 0 \; \vee \; 4x^{2} + 4y^{2} + 6xy = 0 \\
& \implies x = 0 \; \vee \; y = 0 \; \vee \; (x = 0 \; \wedge \; y = 0)
\end{aligned}
$$


(d) 
$$
\begin{aligned}
TBD
\end{aligned}
$$
