---
solver: "Ileumassamuel"
date: "2021-08-30"
exerciseNumber: "1-18"

edition: "4"
author: "Michael Spivak"
textbook: "Calculus"
---

An exercise consisting of proofs.

(a) Let's begin by testing the first number. 
$$
\begin{aligned}
x^{2} + bx + c = 0 & \implies (\frac{-b + \sqrt{b^{2} -4c}}{2})^{2} + b\frac{-b + \sqrt{b^{2} -4c}}{2} + c = 0 \\
& \implies \frac{(-b + \sqrt{b^{2} -4c})^{2} }{4} + \frac{-b^{2} + b\sqrt{b^{2} -4c}}{2} + c = 0 \\
& \implies \frac{b^{2} - 2b\sqrt{b^{2} -4c} + (b^{2} -4c) }{4} + \frac{-2b^{2} + 2b\sqrt{b^{2} - 4c}}{4} + c = 0 \\
& \implies \frac{-4c}{4} + c = 0 \\
& \implies -c + c = 0 \\
& \implies 0 = 0
\end{aligned}
$$


Moving on to the second number, 
$$
\begin{aligned}
x^{2} + bx + c = 0 & \implies (\frac{-b - \sqrt{b^{2} -4c}}{2})^{2} + b\frac{-b - \sqrt{b^{2} -4c}}{2} + c = 0 \\
& \implies \frac{(-b - \sqrt{b^{2} -4c})^{2} }{4} + \frac{-b^{2} - b\sqrt{b^{2} -4c}}{2} + c = 0 \\
& \implies \frac{b^{2} + 2b\sqrt{b^{2} -4c} + (b^{2} -4c) }{4} + \frac{-2b^{2} - 2b\sqrt{b^{2} - 4c}}{4} + c = 0 \\
& \implies \frac{-4c}{4} + c = 0 \\
& \implies -c + c = 0 \\
& \implies 0 = 0
\end{aligned}
$$


(b) We use a proof by contradiction. 
$$
\begin{aligned}
x^{2} + bx + c = 0 & \implies x^{2} + bx + \frac{b^{2}}{4} - \frac{b^{2}}{4} + c = 0 \\
& \implies (x + \frac{b}{2})^{2} - \frac{b^{2}}{4} + c = 0 \\
& \implies (x + \frac{b}{2})^{2} = \frac{b^{2}}{4} - c \\
& \implies 4(x + \frac{b}{2})^{2} = b^{2} - 4c < 0 \\
& \implies 4(x + \frac{b}{2})^{2} < 0 \\
& \implies (x + \frac{b}{2})^{2} < 0
\end{aligned}
$$


We thus end up with a contradiction since any number squared is
greater or equal to 0.

(c) 
$$
\begin{aligned}
b^{2} - 4c < 0 & \implies b^{2} < 4c \\
& \implies y^{2} < 4y^{2} && b = y \wedge c = y^{2} \\
& \implies x^{2} + yx + y^{2} > 0 && \text{Using b}
\end{aligned}
$$


(d) We first need to prove another proposition:

$$
a^{2} < b \; \wedge \; b > 0 \implies -\sqrt{b} < a < \sqrt{b}
$$


$$
\begin{aligned}
a^{2} < b & \implies b > a^{2} \\
& \implies b - a^{2} > 0 \\
& \implies (\sqrt{b} - a)(\sqrt{b} + a) > 0 \\
& \implies [ \sqrt{b} - a > 0 \; \wedge \; \sqrt{b} + a > 0 ] \; \vee \; [ \sqrt{b} - a < 0 \; \wedge \; \sqrt{b} + a < 0 ] \\
& \implies [ \sqrt{b} > a \; \wedge \; \sqrt{a} > -b ] \; \vee \; [ \sqrt{b} < a \; \wedge \; \sqrt{b}  < -a ] \\
& \implies -\sqrt{b} < a < \sqrt{b}
\end{aligned}
$$


Now, we can prove the main proposition. 
$$
\begin{aligned}
b^{2} - 4c < 0 & \implies {(\alpha y)}^{2} - 4y^{2} < 0 && b = \alpha y \wedge c = y^{2} \\
& \implies \alpha^{2}y^{2} < 4y^{2} \\
& \implies \alpha^{2} < 4 \\
& \implies -2 < \alpha < 2 && \text{Proved prop.}
\end{aligned}
$$


(e) For $x^{2} + bx + c$, using the factorization done in (b), the
quadratic is at least equal to $-\frac{b^{2}}{4} + c$.

For $ax^{2} + bx + c$, we factorize it like we factorized the
equation in (b), so as to create a perfect square and a constant
side term. 
$$
\begin{aligned}
ax^{2} + bx + c &= a (x^{2} + \frac{bx}{a}) + c \\
&= a (x^{2} + \frac{bx}{a} + (\frac{b}{2a})^{2}) - (\frac{b}{2a})^{2}) ) + c \\
&= a ( (x + \frac{b}{2a})^{2} - \frac{b^{2}}{4a^{2}} ) + c \\
&= a(x + \frac{b}{2a})^{2} - a \frac{b^{2}}{4a^{2}} + c \\
&= a(x + \frac{b}{2a})^{2} - \frac{b^{2}}{4a} + c
\end{aligned}
$$


Thus, the smallest possible value of $ax^{2} + bx + c$ is
$- \frac{b^{2}}{4a} + c$
