---
solver: "Ileumassamuel"
date: "2021-08-30"
exerciseNumber: "1-19"

edition: "4"
author: "Michael Spivak"
textbook: "Calculus"
---

Behold, the Schwartz inequality. 
$$
\begin{aligned}
x_{1}y_{1} + x_{2}y_{2} \leq \sqrt{x_{1}^{2} + x_{2}^{2} }\sqrt{y_{1}^{2} + y_{2}^{2}}
\end{aligned}
$$


(a) 
$$
\begin{aligned}
x_{1}y_{1} + x_{2}y_{2} &= (\lambda y_{1}) y_{1} + (\lambda y_{2}) y_{2} \\
&= \lambda y_{1}^{2} + \lambda y_{2}^{2} \\
&= \sqrt{ {(\lambda y_{1}) }^{2} + {(\lambda y_{2})}^{2} } \sqrt{y_{1}^{2} + y_{2}^{2}} \\
&= \sqrt{\lambda^{2} y_{1}^{2} + \lambda^{2} y_{2}^{2} } \sqrt{y_{1}^{2} + y_{2}^{2}} \\
&= \sqrt{\lambda^{2} (y_{1}^{2} + y_{2}^{2})} \sqrt{y_{1}^{2} + y_{2}^{2}} \\
&= \sqrt{\lambda^{2} {(y_{1}^{2} + y_{2}^{2})}^{2} } \\
&= \lambda(y_{1}^{2} + y_{2}^{2}) \\
&= \lambda y_{1}^{2} + \lambda y_{2}^{2}
\end{aligned}
$$


Now, if $y_{1} = y_{2} = 0$. 
$$
\begin{aligned}
x_{1} \cdot 0 + x_{2} \cdot 0 &= \sqrt{x_{1}^{2} + x_{2}^{2}} \sqrt{0^{2} + 0^{2}} \\
&= 0
\end{aligned}
$$
