---
solver: "Ileumassamuel"
date: "2021-08-30"
exerciseNumber: "1-20"

edition: "4"
author: "Michael Spivak"
textbook: "Calculus"
---

Summing both inequalities seems to be able to make a
triangle inequality appear. That's what we will try. 
$$
\begin{aligned}
|x - x_{0} | + |y - y_{0}| < \frac{\epsilon}{2} + \frac{\epsilon}{2}
& \implies |x - x_{0} | + |y - y_{0}| < \epsilon && 1.5.i \\
& \implies |(x - x_{0}) + (y - y_{0})| \leq |x - x_{0} | + |y - y_{0}| < \epsilon \\
& \implies |(x - x_{0}) + (y - y_{0})| < \epsilon \\
& \implies |(x + y) - (x_{0} + y_{0})| < \epsilon
\end{aligned}
$$


The second inequality looks similar to the first one, but its inspection
implicitly reveals us that, if we are to use the triangle inequality
once again, the second term needs to be $y_{0} - y$ instead of
$y - y_{0}$. 
$$
\begin{aligned}
|y - y_{0} | < \frac{\epsilon}{2} & \implies |y_{0} - y| < \frac{\epsilon}{2} && 1.14.a \\
& \implies |x - x_{0} | + |y_{0} - y| < \epsilon && 1.5.i \\
& \implies |(x - x_{0}) + (y_{0} - y)| \leq |x - x_{0} | + |y_{0} - y| < \epsilon \\
& \implies |(x - x_{0}) + (y_{0} - y)| < \epsilon \\
& \implies |(x - y) - (x_{0} - y_{0})| < \epsilon
\end{aligned}
$$


# Numbers of various sorts
