---
solver: "Ileumassamuel"
date: "2021-08-30"
exerciseNumber: "1-3"

edition: "4"
author: "Michael Spivak"
textbook: "Calculus"
---

(i) 
$$
\begin{aligned}
\frac{a}{b} &= a b^{-1} \\
&= ab^{-1} \cdot 1 \\
&= ab^{-1} \cdot c c^{-1} \\
&= ac \cdot b^{-1} c^{-1} \\
&= ac {(bc)}^{-1} \\
&= \frac{ac}{bc}
\end{aligned}
$$


(ii) 
$$
\begin{aligned}
\frac{a}{b} + \frac{c}{d} & = a b^{-1} + c d^{-1} \\
&= ab^{-1} \cdot 1 + cd^{-1} \cdot 1 \\
&= ab^{-1} \cdot d d^{-1} + cd^{-1} \cdot bb^{-1} \\
&= ad b^{-1} d^{-1} + bc b^{-1}d^{-1} && \text{Commutativity} \\
&= ad {(bd)}^{-1} + bc {(bd)}^{-1} && (i) \\
&= (ad + bc){(bd)}^{-1} && \text{Distributivity} \\
&= \frac{ad + bc}{bd}
\end{aligned}
$$


(iii) 
$$
\begin{aligned}
a, b \neq 0 & \implies ab \neq 0 \\
& \implies \exists \ {(ab)}^{-1} \\
& \implies {(ab)}^{-1}
= {(ab)}^{-1} \cdot 1 \cdot 1
= {(ab)}^{-1} \cdot aa^{-1} \cdot bb^{-1}
= {(ab)}^{-1} (ab) a^{-1} b^{-1}
= a^{-1} b^{-1}
\end{aligned}
$$


(iv) 
$$
\begin{aligned}
b, d \neq 0 & \implies \exists \ b^{-1}, d^{-1} \\
& \implies \frac{a}{b} \cdot \frac{c}{d} 
= a b^{-1} \cdot c d^{-1} 
= ac \cdot b^{-1} d^{-1}
= ac \cdot (bd)^{-1}
= \frac{ac}{bd} && (iii)
\end{aligned}
$$


(v) We first need to prove that ${(a^{-1})}^{-1} = a$ 
$$
\begin{aligned}
{(a^{-1})}^{-1} &= {(a^{-1})}^{-1} \cdot 1 \\
&= {(a^{-1})}^{-1} \cdot (a a^{-1}) \\
&= {(a^{-1})}^{-1} \cdot a^{-1} \cdot a && \text{Commutativity} \\
&= a
\end{aligned}
$$


We can then go on and prove the actual exercise: 
$$
\begin{aligned}
b, c, d \neq 0 & \implies \exists \ b^{-1}, c^{-1}, d^{-1} \\
& \implies \frac{a}{b} / \frac{c}{d}
= a b^{-1} {(c d^{-1})}^{-1}
= a b^{-1} c^{-1} {(d^{-1})}^{-1}
= a b^{-1} c^{-1} d
= ad {(bc)}^{-1}
= \frac{ad}{bc}
\end{aligned}
$$


(vi) 
$$
\begin{aligned}
\frac{a}{b} = \frac{c}{d} & \iff a b^{-1} = c d^{-1} \\
& \iff a b^{-1} (b d) = c d^{-1} (b d) \\
& \iff a (b^{-1} b) d = c(d^{-1}d)b && \text{Associativity and Commutativity} \\
& \iff ad = bc
\end{aligned}
$$
