---
solver: "Ileumassamuel"
date: "2021-08-30"
exerciseNumber: "1-5"

edition: "4"
author: "Michael Spivak"
textbook: "Calculus"
---

(i) 
$$
\begin{aligned}
a < b \ \wedge \ c < d & \implies b - a > 0 \ \wedge \ d - c > 0 \\
& \implies (b - a) + (d - c) > 0 && \text{Closure under addition} \\ 
& \implies b + d > a + c \\
& \implies a + c < b + d && \text{By definition}
\end{aligned}
$$


(ii) 
$$
\begin{aligned}
a < b & \implies b - a \in P && \text{By definition} \\
& \implies - a + b \in P \\
& \implies - a + b > 0 \\
& \implies - a > - b
\end{aligned}
$$


(iii) 
$$
\begin{aligned}
a < b & \implies b - a \in P \\
& \implies (b - a) \times c \in P && \text{Closure under multiplication} \\
& \implies (b - a) c > 0 \\
& \implies bc - ac > 0 \\
& \implies bc > ac \\
& \implies ac < bc
\end{aligned}
$$


(iv) We first notice that: 
$$
\begin{aligned}
c < 0 & \implies c \in -P \\
& \implies -c \in P
\end{aligned}
$$


Then, 
$$
\begin{aligned}
a < b & \implies b - a \in P \\
& \implies (b - a) \times -c \in P && \text{Closure under multiplication} \\
& \implies (b - a) (-c) > 0 \\
& \implies -bc + ac > 0 \\
& \implies ac > bc
\end{aligned}
$$


(v) 
$$
\begin{aligned}
a > 1 & \implies a - 1 \in P \\
& \implies (a - 1) \times a \in P && \text{Closure under multiplication} \\
& \implies (a - 1) a > 0 \\
& \implies a^2 - a > 0 \\
& \implies a^2 > a 
\end{aligned}
$$


(vi) 
$$
\begin{aligned}
0 < a < 1 & \implies a \in P \ \wedge \ 1 - a \in P \\
& \implies (1 - a) a \in P && \text{Closure under multiplication} \\
& \implies (1 - a) a > 0 \\
& \implies a - a^2 > 0 \\
& \implies a > a^2 \\
& \implies a^2 < a
\end{aligned}
$$


(vii) 
$$
\begin{aligned}
b - a, c \in P \ \wedge \ d - c, b \in P & \implies (b - a) c \in P \ \wedge \ (d - c) b \\
& \implies bc - ac \in P \ \wedge \ bd - bc \in P \\
& \implies bc > ac \ \wedge \ bd > bc \\
& \implies bd > ac && \text{By the transitivity property}
\end{aligned}
$$


(viii) 
$$
\begin{aligned}
0 \leq a < b \ \wedge \ 0 \leq a < b & \implies a^2 < b^2 && \text{Using 9}, c = a, b = d
\end{aligned}
$$


(ix) 
$$
\begin{aligned}
a^2 < b^2 & \implies b^2 - a^2 \in P \\
& \implies (b - a) (b + a) \in P && \text{Square completion} \\
& \implies [\; b - a, b + a \in P \;] \vee [\; - (b - a), -(b + a) \in P \;]
\end{aligned}
$$


Notice that the second case would lead to a contradiction with the
initial premise that $a, b \geq 0$, so we ignore it. With some
simple algebraic manipulation, we obtain: 
$$
\begin{aligned}
b - a > 0 \ \wedge \ b + a > 0 & \implies b > a \ \wedge \ b > -a \\
& \implies a < b && \text{Ignoring the second inequality}
\end{aligned}
$$
