---
solver: "Ileumassamuel"
date: "2021-08-30"
exerciseNumber: "1-9"

edition: "4"
author: "Michael Spivak"
textbook: "Calculus"
---

(i) 
$$
\begin{aligned}
\sqrt{7} > \sqrt{5} & \implies \sqrt{7} - \sqrt{5} > 0 \\
& \implies \sqrt{2} + \sqrt{3} + (\sqrt{7} - \sqrt{5}) > 0 \\
& \implies | \sqrt{2} + \sqrt{3} - \sqrt{5} + \sqrt{7} | = \sqrt{2} + \sqrt{3} - \sqrt{5} + \sqrt{7} > 0
\end{aligned}
$$


**NB.** We us the proposition that the square root function is
strictly increasing.

(ii) 
$$
\begin{aligned}
|a + b| \leq |a| + |b| & \implies |a + b| - |a| - |b| \leq 0 && \text{Triangle inequality} \\
& \implies |a| + |b| - |a + b| \geq 0 \\
& \implies -(|a + b| - |a| - |b|) \geq 0 \\
& \implies ||a + b| - |a| - |b|| = -(|a + b| - |a| - |b|) \geq 0
\end{aligned}
$$


(iii) For this exercise, one might be tempted to treat multiple cases
for the variables, and try to prove that a certain pair/pairs of
absolute values can be removed.

**There is an easier way, however**. What happens when we
substitute our sum $a + b$ with an arbitrary variable. In other
words, let $d = a + b$. Then, 
$$
\begin{aligned}
|a + b| + |c| - |a + b + c| & \implies |d| + |c| - |d + c| \\
& \implies |d + c| \leq |d| + |c| \\
& \implies 0 \leq |d| + |c| - |d + c| \\
& \implies ||a + b| + |c| - |a + b + c|| = |a + b| + |c| - |a + b + c| \geq 0
\end{aligned}
$$


(iv) 
$$
\begin{aligned}
|{ (x - y) }^{2}| = { (x - y) }^{2} = x^{2} - 2xy + y^{2} && \text{Perfect square}
\end{aligned}
$$


(v) 
$$
\begin{aligned}
|( \sqrt{2} + \sqrt{3} - (-(\sqrt{5} - \sqrt{7})) )|
\end{aligned}
$$
