---
solver: "Ileumassamuel"
date: "2021-08-30"
exerciseNumber: "2-1"

edition: "4"
author: "Michael Spivak"
textbook: "Calculus"
---

(i) We begin by proving that the base case holds; that the equality
holds for $n = 1$. 
$$
\begin{aligned}
1^{2} &= \frac{1 (1 + 1)(2 \cdot 1 + 1)}{6} \\
&= \frac{1 \cdot 2 \cdot 3}{6} \\
&= \frac{6}{6} \\
&= 1
\end{aligned}
$$


We then prove that the equation holds for $n+1$, if it holds for
$n$. 
$$
\begin{aligned}
1^{2} + \dots + {(n + 1)}^{2} &= \frac{n(n+1)(2n+1)}{6} + {(n + 1)}^{2} \\
&= \frac{n(n+1)(2n+1)}{6} + \frac{6 {(n + 1)}^{2} }{6} \\
&= \frac{(n + 1)(n(2n + 1) + 6(n + 1))}{6} \\
&= \frac{(n + 1)(2n^{2} + n + 6n + 6)}{6} \\
&= \frac{(n + 1)(2n^{2} + 7n + 6)}{6} \\
&= \frac{(n + 1)(2n^{2} + 4n + 3n + 6)}{6} \\
&= \frac{(n + 1)(2n(n + 2) + 3 (n + 2))}{6} \\
&= \frac{(n + 1)((2n + 3)(n + 2))}{6} \\
&= \frac{(n + 1)(2n + 3)(n + 2)}{6}
\end{aligned}
$$


(ii) Again, we begin by proving the base case. 
$$
\begin{aligned}
1^{3} &= {(1)}^{2} \\
&= 1
\end{aligned}
$$


We then move on to prove that the equation holds for $n + 1$, if it
holds for $n$. 
$$
\begin{aligned}
1^{3} + \dots + {(n + 1)}^{3} &= {(1 + \dots + n)}^{2} + {(n + 1)}^{3} \\
&= ( \frac{n (n + 1)}{2} )^{2} + (n + 1)^{3} \\
&= \frac{n^{2} (n + 1)^{2} }{4} + \frac{4(n + 1)^{3}}{4} \\
&= \frac{(n + 1)^{2} (n^{2} + 4 (n + 1))}{4} \\
&= \frac{(n + 1)^{2} (n^{2} + 4n + 4)}{4} \\
&= \frac{(n + 1)^{2} (n + 2)^{2} }{4} \\
&= (\frac{(n + 1)(n + 2)}{2})^{2} \\
&= (1 + \dots + (n + 1) )^{2}
\end{aligned}
$$
