---
solver: "Ileumassamuel"
date: "2021-08-30"
exerciseNumber: "2-3"

edition: "4"
author: "Michael Spivak"
textbook: "Calculus"
---

If $0 \leq k \leq n$, the \"binomial coefficient\"
$\binom{n}{k}$ is defined by 
$$
\begin{aligned}
& \binom{n}{k} = \frac{n!}{k! (n - k)!}, \qquad \text{if } k \neq 0 \qquad
\text{where } n! = n (n - 1) \cdots 2 \cdot 1 \\
& \binom{n}{0} = \binom{n}{n} = 1
\end{aligned}
$$


(a) 
$$
\begin{aligned}
{n\choose{k - 1}} + {n\choose{k}} &= \frac{n!}{(k - 1)! (n - (k - 1)! )} + \frac{n!}{k!(n - k)!} \\
&= \frac{n! \cdot k}{k(k - 1)! (n - k + 1)! } + \frac{n! \cdot (n - k + 1)}{k!(n - k + 1)(n - k)!} \\
&= \frac{n! \cdot k}{k! (n - k + 1)! } + \frac{n! \cdot (n - k + 1)}{k!(n - k + 1)!} \\
&= \frac{n! (k + (n - k + 1))}{k! (n - k + 1)!} \\
&= \frac{n! (n + 1)}{k! (n + 1 - k )!} \\
&= \frac{(n + 1)! }{k! ((n + 1) - k)!} \\
&= {n + 1 \choose{k}}
\end{aligned}
$$


(b) Inducting on $n$, we would have to prove the base case:

$$
\begin{aligned}
{1\choose{k}} \qquad k \in \mathbb{N}: 0 \leq k \leq 1
\end{aligned}
$$


Then, we need to prove the induction step, using the equation in
(a). 
$$
\begin{aligned}
{n + 1 \choose{k}} = {n \choose{k - 1}} + {n \choose{k}}
\end{aligned}
$$


(c) Give another proof for $n\choose{k}$

(d) Prove the binomial theorem.

Let us start by proving the base case 
$$
\begin{aligned}
(a + b)^{0} &= \sum_{k = 0}^{0} {0 \choose{0}} a^{k}b^{0 - k} \\
&= {0 \choose{0}} a^{0} b^{0} \\
&= 1
\end{aligned}
$$


Moving on to inducting on n, 
$$
\begin{aligned}
{(a + b)}^{n + 1} &= {(a + b)}^{n} (a + b) \\
&= ( \sum_{k = 0}^{n} {n\choose{k}} a^{k} b^{n - k}) (a + b) \\
&= a \sum_{k = 0}^{n} {n\choose{k}} a^{k} b^{n - k}
+ b \sum_{k = 0}^{n} {n\choose{k}} a^{k} b^{n - k} \\
&= \sum_{k = 0}^{n} {n\choose{k}} a^{k + 1} b^{n - k}
+ \sum_{k = 0}^{n} {n\choose{k}} a^{k} b^{n + 1 - k} \\
&= {n\choose{n}}a^{n + 1}b^{n - n} + {n\choose{0}}a^{0}b^{n - 0 + 1}
+ \sum_{k = 0}^{n - 1} {n\choose{k}} a^{k + 1} b^{n - k}
+ \sum_{k = 1}^{n} {n\choose{k}} a^{k} b^{n + 1 - k} \\
&= a^{n + 1} + b^{n + 1}
+ \sum_{k = 0}^{n - 1} {n\choose{k}} a^{k + 1} b^{n - k}
+ \sum_{k = 1}^{n} {n\choose{k}} a^{k} b^{n + 1 - k} \\
&= a^{n + 1} + b^{n + 1}
+ \sum_{k = 1}^{n} {n\choose{k - 1}} a^{k} b^{n + 1 - k}
+ \sum_{k = 1}^{n} {n\choose{k}} a^{k} b^{n + 1 - k} \\
&= a^{n + 1} + b^{n + 1}
+ \sum_{k = 1}^{n} a^{k} b^{n + 1 - k} ({n\choose{k - 1}} + {n\choose{k}}) \\
&= a^{n + 1} + b^{n + 1}
+ \sum_{k = 1}^{n} a^{k} b^{n + 1 - k} {n + 1\choose{k}} \\
&= \sum_{k = 0}^{n + 1} {n + 1\choose{k}} a^{k} b^{n + 1 - k} 
\end{aligned}
$$


(e) (i) 
$$
\begin{aligned}
\sum_{j = 0}^{n} {n\choose{j}} &= \sum_{j = 0}^{n} {n\choose{j}} 1^{j} 1^{n - j} \\
&= (1 + 1)^{n} \\
&= 2^{n}
\end{aligned}
$$


(ii) 
$$
\begin{aligned}
\sum_{j = 0}^{n} (-1)^{j} {n\choose{j}} &= \sum_{j = 0}^{n} (-1)^{j} 1^{n - j} {n\choose{j}} \\
&= {((-1) + 1)}^{n} \\
&= {0}^{n} \\
&= 0
\end{aligned}
$$


(iii) Notice that we almost obtain the partial sum we desire by
subtracting equation (ii) from equation (i). We need to,
however, handle the two possible cases of $n$. Starting with
when $n$ is odd, 
$$
\begin{aligned}
( & {n\choose{0}} + {n\choose{1}} + \dots + {n\choose{n - 1}} + {n\choose{n}}) -
({n\choose{0}} - {n\choose{1}} + \dots - {n\choose{n}}) \\
&= ({n\choose{0}} - {n\choose{0}}) + ({n\choose{1}} + {n\choose{1}}) + \dots + ({n\choose{n - 1}} - {n\choose{n - 1}}) + ({n\choose{n}} + {n\choose{n}}) \\
&= 2{n\choose{1}} + 2{n\choose{3}} + \dots + 2 {n\choose{n}}
\end{aligned}
$$


It then only is a matter of replacing the difference by both
formulas and dividing by 2: 
$$
\begin{aligned}
\frac{\sum_{j = 0}^{n} {n\choose{j}} - \sum_{j = 0}^{n} (-1)^{j} {n\choose{j}}}{2}
&= \frac{2{n\choose{1}} + 2{n\choose{3}} + \dots + 2 {n\choose{n}}}{2} \\
&= {n\choose{1}} + {n\choose{3}} + \dots + {n\choose{n}} \\
&= \frac{2^{n} - 0}{2} \\
&= 2^{n - 1}
\end{aligned}
$$


The other case where $n$ is even is left as an exercise.

(iv) 
$$
\begin{aligned}
{n\choose{0}} + {n\choose{2}} + \dots &= \sum_{j = 0}^{n} {n\choose{j}} - \sum_{\text{l odd}}^{n} {n\choose{l}} \\
&= 2^{n} - 2^{n - 1} \\
&= 2^{n - 1}(2 - 1) \\
& = 2^{n - 1}
\end{aligned}
$$
