---
solver: "Ileumassamuel"
date: "2021-08-30"
exerciseNumber: "2-4"

edition: "4"
author: "Michael Spivak"
textbook: "Calculus"
---

(a) Let's begin by applying the suggested hint. 
$$
\begin{aligned}
{(1 + x)}^{n} ({1 + x})^{m}
&= \sum_{i = 0}^{n} {n\choose{i}} x^{i} 1^{n - i} \sum_{j = 0}^{m} {m\choose{j}} x^{j} 1^{m - j} \\
&= \sum_{i = 0}^{n} {n\choose{i}} x^{i} \sum_{j = 0}^{m} {m\choose{j}} x^{j} \\
&= ( {n\choose{0}} + {n\choose{1}}x^{1} + \dots + {n\choose{n}}x^{n} ) \\
& \quad \times ( {m\choose{0}} + {m\choose{1}}x^{1} + \dots + {m\choose{m}}x^{m} )
\end{aligned}
$$
Notice, also, that
${(1 + x)}^{n}{(1 + x)}^{m} = {(1 + x)}^{n + m}$. Thus,

$$
\begin{aligned}
{(1 + x)}^{n} ({1 + x})^{m} &= {(1 + x)}^{n + m} \\
&= \sum_{l = 0}^{n + m} {n + m \choose{l}} x^{l} \\
&= {n + m \choose{0}} + {n + m \choose{1}} x^{1} + \dots + {n + m \choose{n + m}}x^{n + m}
\end{aligned}
$$
Now, by applying distributivity on the
first equation: 
$$
\begin{aligned}
( & {n\choose{0}} + {n\choose{1}}x^{1} + \dots + {n\choose{n}}x^{n} )
\times ( {m\choose{0}} + {m\choose{1}}x^{1} + \dots + {m\choose{m}}x^{m} ) \\
&= {n\choose{0}} ({m\choose{0}} + \dots + {m\choose{m}}x^{m}) + \dots + {n\choose{n}} ({m\choose{0}} + \dots + {m\choose{m}}x^{m}) \\
&= ({n\choose{0}} {m\choose{0}}) + ( {n\choose{0}} {m\choose{1}}x^{1} + {n\choose{1}}x^{1} {m\choose{0}})
+ \dots + ({n\choose{n}}x^{n} {m\choose{m}}x^{m} ) \\
&= ({n\choose{0}} {m\choose{0}}) + ( {n\choose{0}} {m\choose{1}} + {n\choose{1}} {m\choose{0}})x^{1}
+ \dots + {n + m \choose{n + m}}x^{n + m}
\end{aligned}
$$
By equating the two, we obtain:

$$
\begin{aligned}
( & {n\choose{0}} {m\choose{0}}) + ( {n\choose{0}} {m\choose{1}} + {n\choose{1}} {m\choose{0}})x^{1}
+ \dots + {n + m \choose{n + m}}x^{n + m} \\
&= {n + m \choose{0}} + {n + m \choose{1}} x^{1} + \dots + {n + m \choose{n + m}}x^{n + m} \\
&\implies \sum_{k = 0}^{l} {n\choose{k}} {m\choose{l - k}} = {n + m \choose{l}}
\end{aligned}
$$


(b) 
$$
\begin{aligned}
{2n\choose{n}} &= {n + n \choose{n}} \\
&= \sum_{k = 0}^{n} {n\choose{k}} {n\choose{n - k}} && (a) \\
&= \sum_{k = 0}^{n} {n\choose{k}}^{2} && {n\choose{k}} = {n\choose{n - k}}
\end{aligned}
$$
