---
solver: "Ileumassamuel"
date: "2021-08-30"
exerciseNumber: "2-5"

edition: "4"
author: "Michael Spivak"
textbook: "Calculus"
---

(a) Let us first prove the base case $n = 0$. 
$$
\begin{aligned}
n = 0 \implies 1 &= \frac{1 - r^{0 + 1}}{1 - r} \\
&= \frac{1 - r}{1 - r} \\
&= 1
\end{aligned}
$$


Moving on, we prove that the predicate holds for $n + 1$ if it does
for $n$. 
$$
\begin{aligned}
1 + r + r^{2} + \dots + r^{n} + r^{n + 1} &= \frac{1 - r^{n + 1}}{1 - r} + r^{n + 1} \\
&= \frac{1 - r^{n + 1}}{1 - r} + \frac{(1 - r) r^{n + 1}}{1 - r} \\
&= \frac{1 - r^{n + 1} + r^{n + 1} - r^{n + 2}}{1 - r} \\
&= \frac{1 - r^{n + 2}}{1 - r}
\end{aligned}
$$


(b) 
$$
\begin{aligned}
S (1 - r) &= S - Sr \\
&= 1 + r + \dots + r^{n} - (r + r^{2} + \dots + r^{n} + r^{n + 1}) \\
&= 1 - r^{n + 1} \\
& \implies S = \frac{1 - r^{n + 1}}{1 - r}
\end{aligned}
$$
