---
solver: "Ileumassamuel"
date: "2021-08-30"
exerciseNumber: "2-3-11"

edition: "2"
author: "Stephen Abbott"
textbook: "Understanding Analysis"
---

(a) Consider a sequence $x_{n}$ that converges to $x$ and another
sequence 
$$
y_{n} = \frac{x_1 + x_2 + \dots + x_{n}}{n}.
$$


By definition, for any $\epsilon > 0$,

$$
\exists N_1 \in \mathbb{N}, \forall n \in \mathbb{N}, \quad n \geq N_1 \implies
\abs{x_{n} - x} < \epsilon.
$$


Let's use the $N_1$ from that definition, for any given $\epsilon$.
Then, consider the absolute difference 
$$
\begin{aligned}
\abs{y_{n} - x} 
&= \abs{\frac{x_1 + x_2 + \dots + x_{n}}{n} - x} \\
&= \abs{\frac{x_1 + x_2 + \dots + x_{n}}{n} -
\frac{xn}{n}} \\
&= \abs{\frac{(x_1 - x) + (x_2 - x) + \dots + (x_{n} -
x)}{n}} \\
&= \abs{ \frac{1}{n}\sum^{N_1 - 1}_{i=1} (x_{i} - x) +
\frac{1}{n}\sum^{n}_{i=N_1} (x_{i} - x)}
\end{aligned}
$$
for $n \geq N_1$. By separating
the sum into two parts, we first apply the triangle inequality and
then find bounds on both parts, hoping they can be strictly inferior
to $\epsilon$ (to satisfy the definition of convergence). Thus,

$$
\abs{ \frac{1}{n}\sum^{N_1 - 1}_{i=1} (x_{i} - x) +
\frac{1}{n}\sum^{n}_{i=N_1} (x_{i} - x)}
\leq \frac{1}{n} \sum^{N_1 - 1}_{i=1} \abs{x_{i} - x} +
\frac{1}{n} \sum^{n}_{i=N_1} \abs{x_{i} - x}
$$


Notice that the first part has a constant numerator but an
increasing denominator, dependent only on $n$. Therefore, by the
Archimedean property, we can find $N_2$ for which

$$
\frac{1}{n} \sum^{N_1 - 1}_{i=1} \abs{x_{i} - x} <
\frac{\epsilon (N_1 - 1)}{N_1}
= \frac{\epsilon N_1}{N_1} - \frac{\epsilon}{N_1}
$$

when $n \geq N_2$. For the second part, notice that all the terms of
the numerator are in $V_{\epsilon}(x)$. Therefore, their sum can be
bounded above by $\epsilon$ because the furthest $x_{n}$ can be from
$x$ in that interval is less than $\epsilon$. Now, if we choose
$N = \max \{N_1, N_2\}$, we obtain 
$$
\begin{aligned}
\abs{y_{n} - x} 
&=\abs{ \frac{1}{n}\sum^{N_1 - 1}_{i=1} (x_{i} - x) +
\frac{1}{n}\sum^{n}_{i=N_1} (x_{i} - x)} \\
&\leq \frac{1}{n}
\sum^{N_1 - 1}_{i=1} \abs{x_{i} - x} + \frac{1}{n}
\sum^{n}_{i=N_1} \abs{x_{i} - x} \\
&< \frac{\epsilon (N_1 - 1)}{N_1} + \frac{1}{n} (n - N_1 +
1) \epsilon \\
&= \frac{\epsilon N_1}{N_1} - \frac{\epsilon}{N_1} +
\epsilon - \frac{\epsilon N}{n} + \frac{\epsilon}{n} \\
&= (\frac{\epsilon N_1}{N_1} -\frac{\epsilon N}{n}) \\
&\leq \epsilon 
\end{aligned}
$$


when $n \geq N$.

(b) Consider the sequence 
$$
x_{n} = (0, 1, 0, 1, \dots).
$$
Clearly, it
does not converge. However, the sequence of its average

$$
y_{n} = (0, \frac{1}{2}, \frac{1}{3}, \frac{2}{4},
\frac{2}{5}, \frac{3}{6}, \dots)
$$
does converge
to 1/2.
