---
solver: "Ileumassamuel"
date: "2021-08-30"
exerciseNumber: "2-3-6"

edition: "2"
author: "Stephen Abbott"
textbook: "Understanding Analysis"
---

By multiplying $b_{n}$ by its conjugate, we obtain an
easier form to deal with. That is, 
$$
b_{n} = n - \sqrt{n^2 + 2n} 
= n - \sqrt{n^2 + 2n} \cdot \frac{n +
\sqrt{n^2 + 2n}}{n + \sqrt{n^2 + 2n}}
= \frac{-2n}{n(1 + \sqrt{1 + \frac{2}{n}})} 
= \frac{-2}{1 + \sqrt{1 + \frac{2}{n}}}
$$


Applying rule (i), we know that 
$$
\lim \frac{2}{n} = 0.
$$
It then
follows with rule (ii) that 
$$
\lim 1 + \frac{2}{n} = 1
$$
and, by
exercise 2.3.1 (b), 
$$
\lim \sqrt{1 + \frac{2}{n}} = \sqrt{1} = 1.
$$

Finally, applying (ii) to 
$$
\lim 1 + \sqrt{1 + \frac{2}{n}}
$$
and (iv)
to $b_{n}$, we obtain

$$
b_{n} = \frac{-2}{1 + \sqrt{1 + \frac{2}{n}}} = -\frac{2}{2} = -1.
$$
