---
solver: "Ileumassamuel"
date: "2021-08-30"
exerciseNumber: "2-3-10"

edition: "2"
author: "Stephen Abbott"
textbook: "Understanding Analysis"
---

(a) **False.** Consider the sequences

$$
a_{n} = b_{n} = (0, 1, 0, 1, \dots).
$$
Clearly the sequence
$( a_{n} - b_{n} )$ converges to 0 (why). However, neither of the
sequences converge.

(b) **True.** By definition, for every $\epsilon > 0$,

$$
\exists N \in \mathbb{N}, \forall n \in \mathbb{N}, \quad n \geq N \implies \abs{b_{n} - b} <
\epsilon.
$$
However, by using the reverse
triangle inequality, we also have

$$
n \geq N \implies \abs{\abs{b_{n}} - \abs{b}} \leq
\abs{b_{n} - b} < \epsilon.
$$


A proof of the reverse triangle inequality is given in the appendix.

(c) **True.** Suppose

$$
a_{n} \rightarrow 0, \quad c_{n} = (b_{n} - a_{n})
\rightarrow 0.
$$
Apply rule (ii) of the
algebraic limit theorem to the limit 
$$
\lim (a_{n} + c_{n})
= \lim a_{n} + \lim c_{n}
= 0 + 0
= 0.
$$
This then implies that $\lim b_{n} = 0$
since 
$$
\lim (a_{n} + c_{n})
= \lim a_{n} + b_{n} - a_{n}
= \lim b_{n}.
$$


(d) **True.** Since

$$
\forall n \in \mathbb{N}, \quad \abs{b_{n} - b} \leq a_{n},
$$

every term of the sequence $a_{n}$ is positive. Therefore, by
definition, for any $\epsilon > 0$,

$$
\exists N \in \mathbb{N}, \forall n \in \mathbb{N}, \quad n \geq N \implies \abs{b_{n} - b}
\leq a_{n} = \abs{a_{n}} < \epsilon.
$$

Therefore, $b_{n}$ converges to $b$.
