---
solver: "Ileumassamuel"
date: "2021-08-30"
exerciseNumber: "2-3-9"

edition: "2"
author: "Stephen Abbott"
textbook: "Understanding Analysis"
---

(a) We are not allowed to use the algebraic limit theorem because there
is no guarantee that $a_{n}$ converges to a given value.

For the actual proof, suppose $a_{n}$ is bounded by $M > 0$ and that
$b_{n}$ converges to 0. By definition, for every $\epsilon
> 0$, we have

$$
\exists N \in \mathbb{N}, \quad n \geq N 
\implies \abs{a_{n}b_{n}} \leq \abs{a_{n}M} <
\frac{\epsilon}{M} M = \epsilon
$$


(b) We do have an example of a sequence $a_{n}b_{n}$ which does not
converge. Suppose 
$$
a_{n} = (0, 1, 0, 1, 0, \dots)
$$
and

$$
b_{n} = (1, 1, 1, 1, \dots).
$$
Obviously $a_{n}$ is bounded by 1
and $b_{n} \rightarrow 1 \neq
0$. However, the sequence $a_{n}b_{n}$ simply is

$$
a_{n}b_{n} = a_{n} =  a_{n} = (0, 1, 0, 1, 0, \dots)
$$
so
$a_{n}b_{n}$ diverges in this case. On the other hand, if $a_{n}$
were equal to $b_{n}$, then our sequence would be convergent (why).
Therefore, it is not possible to establish whether the sequence
$a_{n}b_{n}$ converges or not.

(c) Suppose any sequence $a_{n}$ and $b_{n}$ such that 
$$
\begin{aligned}
a_{n} \rightarrow 0 \\
b_{n} \rightarrow b.
\end{aligned}
$$


Since $b_{n}$ is convergent, it also is bounded then. Therefore we
can apply the proposition from (a) and obtain

$$
\lim a_{n} b_{n} = 0,
$$
thereby proving rule (iii) from the
algebraic limit theorem when $a_{n} \rightarrow 0$.
