---
solver: "Ileumassamuel"
date: "2021-08-30"
exerciseNumber: "2-4-1"

edition: "2"
author: "Stephen Abbott"
textbook: "Understanding Analysis"
---

(a) Since we only need to show that the sequence converges and not find
the actual limit, we can use the Monotone Convergence theorem.

Therefore, we need to prove that the sequence is monotone and
bounded. Let's begin by proving that the sequence is decreasing.
After writing down a few terms, we may come to think that the
sequence is decreasing.

$$
x_{n} = (3, 1, \frac{1}{3}, \frac{3}{11}, \frac{11}{41}, \dots).
$$

To prove that it actually is, we use mathematical induction. The
base case is obviously true since 
$$
1 = x_2 \leq x_1 = 3.
$$


We now prove the induction step by supposing that the statement is
true for the pair $x_{n + 1}, x_{n}$. 
$$
\begin{aligned}
x_{n + 2} - x_{n + 1}
&= \frac{1}{4 - x_{n + 1}} - \frac{1}{4 - x_{n}} \\
&= \frac{(4 - x_{n}) - (4 - x_{n + 1})}{(4 - x_{n + 1}) (4 -
x_{n})} \\
&= \frac{x_{n + 1} - x_{n}}{(4 - x_{n + 1})(4 - x_{n})} > 0
\end{aligned}
$$


(b) Suppose $x_{n}$ is a sequence converging to $x$. Applying the
definition of convergence, any $\epsilon > 0$,

$$
\exists N \in \mathbb{N}, \forall n \in \mathbb{N}, \quad n \geq N
\implies \abs{x_{n} - x} < \epsilon.
$$
This also
implies that for the given $N$,

$$
\forall n \in \mathbb{N}, n \geq N 
\implies \abs{x_{n + 1} - x} < \epsilon.
$$
since
$n + 1 > n$.

(c) Taking the limit on each side, we have 
$$
\begin{aligned}
\lim_{n \to \infty} x_{n} 
&= \lim_{n \to \infty} x_{n + 1} \\
&= \lim_{n \to \infty} \frac{1}{4 - x_{n}}
\end{aligned}
$$


By labeling $\lim_{n \to \infty} x_{n}$ as $L$, we use the algebraic
limit theorem to obtain 
$$
\begin{aligned}
L &= \frac{\lim_{n \to \infty} 1}{\lim_{n \to \infty} 4 -
x_{n}} \\
&= \frac{1}{4 - \lim_{n \to \infty} x_{n}} \\
&= \frac{1}{4 - L}.
\end{aligned}
$$


With some algebraic manipulations, we clearly obtain a quadratic
equation: 
$$
\begin{aligned}
L = \frac{1}{4 - L}
&\implies (4 - L)L = 1 \\
&\implies 4L - L^2 = 1 \\
&\implies -L^2 + 4L - 1 = 0.
\end{aligned}
$$


We can then use the quadratic formula 
$$
\begin{aligned}
\bm{x} &= \frac{-b \pm \sqrt{b^2 - 4ac}}{2a} \\
&= \frac{-4 \pm \sqrt{16 - 4(-1)(-1)}}{2(-1)} \\
&= \frac{-4 \pm \sqrt{12}}{-2} \\
&= 2 \pm \sqrt{3}.
\end{aligned}
$$


Since $x_{n} \leq 3$ for all $n$, the limit cannot be $2 \pm
\sqrt{3} > 3$ and thus is $2 - \sqrt{3}$.
